Phi_Min_ex.thy
@@ -4,9 +4,29 @@ begin
 
 section \<open>Additional Stuffs\<close>
 
-subsection \<open>Convert between Deep Model and Word Type\<close>
+subsection \<open>Representations about Word\<close>
 
-term unat
+subsubsection \<open>Natural Number Abstraction\<close>
+
+paragraph \<open>Natural Number\<close>
+
+definition \<phi>Nat_for_Word :: "('len::len word, nat) \<phi>" ("\<nat>\<^sup>w")
+  where "\<nat>\<^sup>w x = (if x < 2^LENGTH('len) then { of_nat x } else {})"
+
+lemma \<phi>Nat_for_Word_expn[\<phi>expns]:
+  "p \<in> (x \<Ztypecolon> \<nat>\<^sup>w) \<longleftrightarrow> (p = of_nat x) \<and> x < 2^LENGTH('len)" for p :: \<open>'len::len word\<close>
+  unfolding \<phi>Type_def \<phi>Nat_for_Word_def by simp
+
+lemma \<phi>Nat_for_Word_expn_elim[elim!,\<phi>reason_elim!]:
+  "Inhabited (x \<Ztypecolon> \<nat>\<^sup>w :: 'len::len word set) \<Longrightarrow> (x < 2^LENGTH('len) \<Longrightarrow> C) \<Longrightarrow> C"
+  unfolding Inhabited_def by (clarsimp simp add: \<phi>expns)
+
+lemma
+  \<open>Inhabited (x \<Ztypecolon> \<nat>\<^sup>w :: 'len::len word set) \<longleftrightarrow> x < 2^LENGTH('len)\<close>
+  unfolding Inhabited_def by (clarsimp simp add: \<phi>expns)
+
+
+subsubsection \<open>Conversion between Deep representation and Word\<close>
 
 context \<phi>min_sem begin
 
@@ -34,7 +54,7 @@ lemma word_to_V_int_V_int_to_word[simp]:
 
 lemma V_int_to_word_word_to_V_int[simp]:
   \<open>V_int_to_word (word_to_V_int v) = v\<close>
-  unfolding word_to_V_int_def V_int_to_word_def by clarsimp
+  unfolding word_to_V_int_def V_int_to_word_def by clarsimp  
 
 end
 
